Setlec/SetR.lean
@@ -190,6 +190,7 @@ import Setlec.SetR.Interp2.IndRecsP
 import Setlec.SetR.Interp2.ProjRenameP
 import Setlec.SetR.Interp2.ProjConsP
 import Setlec.SetR.Interp2.ProjInstallP
+import Setlec.SetR.Interp2.DeclIndP
 import Setlec.SetR.Interp2.IndPinProbeP
 import Setlec.SetR.Interp2.AxiomPinP
 import Setlec.SetR.Interp2.HarvestP
